glue/generic_falcon_lemmas.dfy
@@ -1,0 +1,93 @@
+include "../spec/bvop/bv_op.s.dfy"
+include "../spec/crypto/falcon512.i.dfy"
+
+abstract module generic_falcon_lemmas {
+    import opened Mul
+    import opened Power
+    import opened DivMod
+    import opened integers
+    import opened pow2_s
+
+    import opened ntt_index
+    import opened falcon_512_i
+
+    import FNTT = falcon_512_i.FNTT
+    import INTT = falcon_512_i.INTT
+    import opened MQP = falcon_512_i.CMQP
+
+    const Q := falcon_512_i.Q;
+    const N := falcon_512_i.N; 
+    const OMEGA := falcon_512_i.CMQ.OMEGA;
+
+    const R := CMQ.R;
+    const PSI := CMQ.PSI;
+
+    type floop_view = FNTT.loop_view
+
+    type iloop_view = INTT.loop_view
+
+    predicate {:opaque} buff_is_n_elems(a: seq<nat>)
+        ensures buff_is_n_elems(a) ==> |a| == N.full;
+    {
+        && (|a| == N.full)
+        && (forall i | 0 <= i < N.full :: a[i] < Q)
+    }
+
+    function {:opaque} buff_as_n_elems(a: seq<nat>): (a': n_elems)
+        requires buff_is_n_elems(a);
+        ensures a == a';
+    {
+        reveal buff_is_n_elems();
+        a
+    }
+
+    function block_size(d: pow2_t): pow2_t
+        requires CPV.block_size.requires(d)
+    {
+        CPV.block_size(d)
+    }
+
+    function build_floop_view(s: n_elems, d: pow2_t): floop_view
+        requires FNTT.build_loop_view.requires(s, d)
+    {
+        FNTT.build_loop_view(s, d)
+    }
+
+    function build_iloop_view(s: n_elems, d: pow2_t): iloop_view
+        requires INTT.build_loop_view.requires(s, d)
+    {
+        INTT.build_loop_view(s, d)
+    }
+
+    function montmul(a: elem, b: elem): elem
+    {
+        MQP.montmul(a, b)
+    }
+
+    function rev_mixed_powers_mont_x_value(i: nat, d: pow2_t): (r: elem)
+    {
+        FNTT.rev_mixed_powers_mont_x_value(i, d)
+    }
+
+    function rev_mixed_powers_mont_table(): n_elems
+    {
+        FNTT.rev_mixed_powers_mont_table()
+    }
+
+    function rev_omega_inv_powers_x_value(i: nat, d: pow2_t): (r: elem)
+    {
+        INTT.rev_omega_inv_powers_x_value(i, d)
+    }
+
+    function rev_omega_inv_powers_mont_table(): n_elems
+    {
+        INTT.rev_omega_inv_powers_mont_table()
+    }
+
+    function inverse_ntt_scaling_table(): n_elems
+    {
+        MQP.inverse_ntt_scaling_table()
+    }
+
+
+}
